src/Model.v
@@ -1,12 +1,13 @@
 Set Warnings "-local-declaration".
 
 Require Import
-  Coq.Classes.Morphisms
   Coq.Program.Program
-  Coq.Sets.Classical_sets
-  Coq.Sets.Ensembles
   Coq.Unicode.Utf8
   Coq.micromega.Lia
+  Coq.Sets.Powerset_facts
+  Coq.Sets.Classical_sets
+  Coq.Sets.Ensembles
+  Coq.Classes.Morphisms
   Same_set
   Stream
   LTL.
@@ -23,12 +24,14 @@ Definition true  := Full_set (Stream a).
 Definition false := Empty_set (Stream a).
 Definition and   := Intersection (Stream a).
 Definition impl  := Included (Stream a).
+Definition eqv   := Same_set (Stream a).
 
 Program Instance impl_reflexive : Reflexive impl.
 Next Obligation.
   unfold impl.
   now repeat intro.
 Qed.
+
 Program Instance impl_transitive : Transitive impl.
 Next Obligation.
   unfold impl, Included in *.
@@ -36,13 +39,234 @@ Next Obligation.
   now intuition.
 Qed.
 
+(* Theorem Inhabited_not x : Inhabited (Stream a) (not x) <-> ~ Inhabited (Stream a) x. *)
+(* Proof. *)
+(*   split; intros. *)
+(*   - destruct H. *)
+(*     intro. *)
+(*     destruct H0. *)
+(*     apply H. *)
+
+Program Instance not_respects_impl : Proper (impl --> impl) not | 1.
+Next Obligation.
+  unfold flip, impl.
+  repeat intro.
+  destruct H0.
+  exists x0.
+  intro.
+  apply H0.
+  now apply H.
+Qed.
+
+Program Instance or_respects_impl : Proper (impl ==> impl ==> impl) or.
+Next Obligation.
+  unfold impl, or.
+  repeat intro.
+  destruct H1; unfold Included, In in *.
+  - left.
+    now apply H.
+  - right.
+    now apply H0.
+Qed.
+
+Program Instance and_respects_impl : Proper (impl ==> impl ==> impl) and.
+Next Obligation.
+  unfold impl, and.
+  repeat intro.
+  destruct H1; unfold Included, In in *.
+  constructor.
+  - now apply H.
+  - now apply H0.
+Qed.
+
+Declare Scope boolean_scope.
+Bind Scope boolean_scope with t.
+Delimit Scope boolean_scope with boolean.
+Open Scope boolean_scope.
+
+Notation "¬ p"    := (not p)    (at level 75, right associativity) : boolean_scope.
+Infix    "∨"      := or         (at level 85, right associativity) : boolean_scope.
+Notation "p ⇒ q"  := (¬ p ∨ q)  (at level 86, right associativity) : boolean_scope.
+Notation "⊤"      := true       (at level 0, no associativity) : boolean_scope.
+Notation "⊥"      := false      (at level 0, no associativity) : boolean_scope.
+Notation "p ⟹ q" := (impl p q) (at level 99, right associativity) : boolean_scope.
+Notation "p ≈ q"  := (eqv p q)  (at level 90, no associativity) : boolean_scope.
+Infix    "∧"       := and             (at level 80, right associativity) : boolean_scope.
+Notation "p ≡ q"   := (p ⇒ q ∧ q ⇒ p) (at level 89, right associativity, only parsing) : boolean_scope.
+
+Theorem eqv_true (p : t) : (p ≈ ⊤) <-> (forall s, p s).
+Proof.
+  split; intros.
+  - apply H.
+    now constructor.
+  - split; repeat intro.
+    + now constructor.
+    + now apply H.
+Qed.
+
+Theorem impl_means (p q : t) : (p ⟹ q) <-> (forall s, p s -> q s).
+Proof.
+  split; intros.
+  - now apply H.
+  - repeat intro.
+    now apply H.
+Qed.
+
+Theorem impl_denote (p q : t) : (p ⟹ q) <-> (p ≈ ⊤ -> q ≈ ⊤).
+Proof.
+  split; intros.
+  - split; repeat intro.
+    + now constructor.
+    + now apply H, H0.
+  - apply impl_means; intros.
+    apply H.
+    + split; intros.
+      * constructor.
+      * repeat intro.
+      apply eqv_true.
+    rewrite H.
+    + now exists p.
+    + split; repeat intro.
+      * now exists p.
+      * destruct H1.
+Admitted.
+
+(** Cannot be proven for sets, so must take it as an axiom in Coq. *)
+Axiom excluded_middle : forall (p : t), Included (Stream a) ⊤ (p ∨ ¬ p).
+
+Theorem true_def (p : t) : p ∨ ¬p ≈ ⊤.
+Proof.
+  split; intros.
+  - constructor.
+  - apply excluded_middle.
+Qed.
+
+Theorem false_def (p : t) : ¬(p ∨ ¬p) ≈ ⊥.
+Proof.
+  split; intros.
+  - rewrite true_def.
+    repeat intro.
+    destruct H.
+    now constructor.
+  - rewrite true_def.
+    repeat intro.
+    contradiction.
+Qed.
+
+Theorem or_comm (p q : t) : p ∨ q ≈ q ∨ p.
+Proof.
+  unfold or.
+  now rewrite Union_commutative.
+Qed.
+
+Theorem or_assoc (p q r : t) : (p ∨ q) ∨ r ≈ p ∨ (q ∨ r).
+Proof.
+  unfold or.
+  now rewrite Union_associative.
+Qed.
+
+Theorem and_def (p q : t) : p ∧ q ≈ ¬(¬p ∨ ¬q).
+Proof.
+  split; repeat intro.
+  - destruct H, H0; contradiction.
+  - admit.
+Admitted.
+
+Theorem huntington (p q : t) : ¬(¬p ∨ ¬q) ∨ ¬(¬p ∨ q) ≈ p.
+Proof.
+  split; intros.
+  - rewrite <- (Complement_Complement _ q) at 2.
+    rewrite <- !and_def.
+    unfold or.
+    rewrite <- Distributivity.
+    rewrite true_def.
+    repeat intro.
+    now destruct H.
+  - rewrite <- (Complement_Complement _ q) at 2.
+    rewrite <- !and_def.
+    unfold or.
+    rewrite <- Distributivity.
+    rewrite true_def.
+    repeat intro.
+    constructor; auto.
+    now constructor.
+Qed.
+
 Definition next : t -> t := λ p s,（s, 1）⊨ p.
 
-Declare Scope ltl_scope.
-Bind Scope ltl_scope with t.
-Open Scope ltl_scope.
+Program Instance next_respects_impl : Proper (impl ==> impl) next.
+Next Obligation.
+  unfold impl, next.
+  repeat intro.
+  apply H, H0.
+Qed.
 
-Notation "◯ p"     := (next p)    (at level 75, right associativity) : ltl_scope.
+Definition until : t -> t -> t :=
+  λ p q s, ∃ k,（s, k）⊨ q /\ ∀ i, i < k ->（s, i）⊨ p.
+
+Program Instance until_respects_impl : Proper (impl ==> impl ==> impl) until.
+Next Obligation.
+  unfold impl, until.
+  repeat intro.
+  destruct H1.
+  exists x2.
+  destruct H1.
+  split.
+  - now apply H0.
+  - intros.
+    apply H.
+    now apply H2.
+Qed.
+
+Theorem (* 1 *) next_not (p : t) : ◯ ¬p ≈ ¬◯ p.
+Theorem (* 2 *) next_impl (p q : t) : ◯ (p ⇒ q) ≈ ◯ p ⇒ ◯ q.
+
+Theorem (* 9 *) next_until (p q : t) : ◯ (p U q) ≈ (◯ p) U (◯ q).
+Theorem (* 10 *) until_expansion (p q : t) : p U q ≈ q ∨ (p ∧ ◯ (p U q)).
+Theorem (* 11 *) until_right_bottom (p : t) : p U ⊥ ≈ ⊥.
+Theorem (* 12 *) until_left_or (p q r : t) : p U (q ∨ r) ≈ (p U q) ∨ (p U r).
+Theorem (* 13 *) until_right_or (p q r : t) : (p U r) ∨ (q U r) ⟹ (p ∨ q) U r.
+Theorem (* 14 *) until_left_and (p q r : t) : p U (q ∧ r) ⟹ (p U q) ∧ (p U r).
+Theorem (* 15 *) until_right_and (p q r : t) : (p ∧ q) U r ≈ (p U r) ∧ (q U r).
+Theorem (* 16 *) until_impl_order (p q r : t) : (p U q) ∧ (¬q U r) ⟹ p U r.
+Theorem (* 17 *) until_right_or_order (p q r : t) : p U (q U r) ⟹ (p ∨ q) U r.
+Theorem (* 18 *) until_right_and_order (p q r : t) : p U (q ∧ r) ⟹ (p U q) U r.
+
+(** jww (2021-02-08): This axiom is just an idea a work in progress *)
+Theorem (* NEW *) until_continue (p q : t) : q ∧ p U ◯ ¬q ⟹ p U (q ∧ ◯ ¬q).
+Theorem (* NEW *) not_until (p q : t) : ⊤ U ¬p ∧ ¬(p U q) ≈ ¬q U (¬p ∧ ¬q).
+
+Definition eventually : t -> t.
+Definition always : t -> t.
+Definition wait : t -> t -> t.
+Definition release : t -> t -> t.
+Definition strong_release : t -> t -> t.
+
+Notation "◇ p"     := (eventually p)       (at level 75, right associativity) : ltl_scope.
+Notation "□ p"     := (always p)           (at level 75, right associativity) : ltl_scope.
+Notation "p 'W' q" := (wait p q)           (at level 79, right associativity) : ltl_scope.
+Notation "p 'R' q" := (release p q)        (at level 79, right associativity) : ltl_scope.
+Notation "p 'M' q" := (strong_release p q) (at level 79, right associativity) : ltl_scope.
+
+Program Instance eventually_respects_impl : Proper (impl ==> impl) eventually.
+Program Instance always_respects_impl : Proper (impl ==> impl) always.
+Program Instance wait_respects_impl : Proper (impl ==> impl ==> impl) wait.
+Program Instance release_respects_impl : Proper (impl ==> impl ==> impl) release.
+Program Instance strong_release_respects_impl : Proper (impl ==> impl ==> impl) strong_release.
+
+Theorem evn_def (p : t) : ◇ p ≈ ⊤ U p.
+Theorem always_def (p : t) : □ p ≈ ¬◇ ¬p.
+Theorem always_until_and_ind (p q r : t) :
+  □ (p ⇒ (◯ p ∧ q) ∨ r) ⟹ p ⇒ □ q ∨ q U r.
+Theorem wait_def (p q : t) : p W q ≈ □ p ∨ p U q.
+Theorem release_def (p q : t) : p R q ≈ ¬(¬p U ¬q).
+Theorem strong_release_def (p q : t) : p M q ≈ p U (q ∧ p).
+
+Include LinearTemporalLogicFacts.
+
+End StreamLTL.
+
+Module StreamLTLFacts.
 
 Theorem next_semantics : ∀ σ j p,（σ, j）⊨ (◯ p) <->（σ, j + 1）⊨ p.
 Proof.
@@ -53,9 +277,6 @@ Proof.
   - rewrite PeanoNat.Nat.add_comm in H.
     now rewrite <- from_plus in H.
 Qed.
-
-Definition until : t -> t -> t :=
-  λ p q s, ∃ k,（s, k）⊨ q /\ ∀ i, i < k ->（s, i）⊨ p.
 
 Notation "p 'U' q" := (until p q) (at level 79, right associativity) : ltl_scope.
 
@@ -97,4 +318,4 @@ Definition eventually : t -> t := λ p s, ∃ i,（s, i）⊨ p.
 Definition wait : t -> t -> t :=
   λ p q s, ∃ k,（s, k）⊨ q /\ ∀ i, i < k ->（s, i）⊨ p.
 
-End StreamLTL.
+End StreamLTLFacts.
